src/spec/properties/TLS13.ConnectionState.ClientCanonicalShape.fst
@@ -608,16 +608,11 @@ let lemma_client_step_facts
           is_client_canonical_event conn_ev))
   = match ev with
     | SM.WireEvent wire ->
-      eliminate exists (msg:M.tls_message).
-        (let conn_ev =
-           CS.ConnNetworkEvent {
-             CL.message_direction = CL.Received;
-             CL.message_value = msg;
-           } in
+      eliminate exists (conn_ev:CS.conn_event).
+        (EC.client_wire_received_event st0 wire conn_ev /\
          SMCan.canonical_wire_step st0 s' conn_ev
            (Common.WireFormat.serialize_all CW.tls_record_wire_format out.SM.so_wire_outputs)
            (CW.wire_serialize wire) /\
-         EC.network_input_message_projection st0 wire msg /\
          EC.client_local_outputs_match conn_ev out.SM.so_local_outputs)
       returns
         (exists (conn_ev:CS.conn_event).
@@ -627,11 +622,6 @@ let lemma_client_step_facts
           is_client_canonical_event conn_ev)
       with _.
       (
-        let conn_ev =
-          CS.ConnNetworkEvent {
-            CL.message_direction = CL.Received;
-            CL.message_value = msg;
-          } in
         assert (is_client_canonical_event conn_ev)
       )
     | SM.LocalEvent local ->
