src/impl/TLS13.Impl.Driver.PairingNoTailWireLogs.fst
@@ -409,12 +409,8 @@ let lemma_client_step_wire_log_delta
 =
   match ev with
   | SM.WireEvent wire ->
-    eliminate exists msg.
-      (let conn_ev =
-        CS.ConnNetworkEvent {
-          CL.message_direction = CL.Received;
-          CL.message_value = msg;
-        } in
+    eliminate exists (conn_ev:CS.conn_event).
+      (EC.client_wire_received_event st0 wire conn_ev /\
       CS.legal_connection_delta
         st0
         {
